RocqOfRust/core/fmt/links/mod.v
@@ -29,32 +29,112 @@ Export (hints) Arguments.
 Module Impl_Arguments.
   Definition Self : Set := Arguments.t.
 
-  (* pub const fn new_const<const N: usize>(pieces: &'a [&'static str; N]) -> Self *)
-  Instance run_new_const
-      (N : usize)
-      (pieces : '& (array.t ('& string) N)) :
-    Run.Trait fmt.Impl_core_fmt_Arguments.new_const [φ N] [] [φ pieces] Self.
-  Proof.
-    constructor.
-    run_symbolic.
+  (* pub unsafe fn new<const N: usize, const M: usize>(
+      template: &'a [u8; N],
+      args: &'a [rt::Argument<'a>; M],
+  ) -> Arguments<'a> *)
+  Instance run_new (N M : usize)
+      (template : '& (array.t u8 N))
+      (args : '& (array.t Argument.t M)) :
+    Run.Trait fmt.Impl_core_fmt_Arguments.new [φ N; φ M] [] [φ template; φ args] Self.
   Admitted.
-  Global Opaque run_new_const.
+  Global Opaque run_new.
 
-  (*
-    pub fn new_v1<const P: usize, const A: usize>(
-        pieces: &'a [&'static str; P],
-        args: &'a [rt::Argument<'a>; A],
-    ) -> Arguments<'a>
-  *)
-  Instance run_new_v1
-      (P A : usize)
-      (pieces : '& (array.t ('& string) P))
-      (args : '& (array.t Argument.t A)) :
-    Run.Trait fmt.Impl_core_fmt_Arguments.new_v1 [φ P; φ A] [] [φ pieces; φ args] Self.
+  Instance run_new_byte_str (N M : usize)
+      (args : '& (array.t Argument.t M)) :
+    Run.Trait
+      fmt.Impl_core_fmt_Arguments.new
+      [φ N; φ M]
+      []
+      [
+        Value.Pointer {|
+          Pointer.kind := Pointer.Kind.Ref;
+          Pointer.core := {|
+            Pointer.kind := Pointer.Kind.Ref;
+            Pointer.core := Pointer.Core.Immediate (Some (
+              Value.Array (repeat_nat
+                (Z.to_nat N.(Integer.value))
+                (Value.Integer IntegerKind.U8 0))
+            ));
+          |}.(Pointer.core);
+        |};
+        φ args
+      ]
+      Self.
+  Proof.
+    replace (
+      Value.Pointer {|
+        Pointer.kind := Pointer.Kind.Ref;
+        Pointer.core := {|
+          Pointer.kind := Pointer.Kind.Ref;
+          Pointer.core := Pointer.Core.Immediate (Some (
+            Value.Array (repeat_nat
+              (Z.to_nat N.(Integer.value))
+              (Value.Integer IntegerKind.U8 0))
+          ));
+        |}.(Pointer.core);
+      |}
+    ) with (
+      φ (Ref.immediate Pointer.Kind.Ref
+        (array.Build_t u8 N
+          (array.ArrayPairs.repeat
+            (Integer.Build_t IntegerKind.U8 0)
+            (Z.to_nat N.(Integer.value)))))
+    ).
+    { apply run_new. }
+    cbn.
+    symmetry.
+    change (
+      Value.Pointer {|
+        Pointer.kind := Pointer.Kind.Ref;
+        Pointer.core := Pointer.Core.Immediate (Some (
+          Value.Array (repeat_nat
+            (Z.to_nat N.(Integer.value))
+            (Value.Integer IntegerKind.U8 0))
+        ));
+      |} =
+      Value.Pointer {|
+        Pointer.kind := Pointer.Kind.Ref;
+        Pointer.core := Pointer.Core.Immediate (Some (
+          Value.Array (array.ArrayPairs.to_values (array.ArrayPairs.repeat
+            (Integer.Build_t IntegerKind.U8 0)
+            (Z.to_nat N.(Integer.value))))
+        ));
+      |}
+    ).
+    do 3 f_equal.
+    f_equal.
+    change (
+      Value.Array
+        (repeat_nat
+          (Z.to_nat N.(Integer.value))
+          (Value.Integer IntegerKind.U8 0)) =
+      φ (array.Build_t u8 N
+        (array.ArrayPairs.repeat
+          (Integer.Build_t IntegerKind.U8 0)
+          (Z.to_nat N.(Integer.value))))
+    ).
+    change (Value.Integer IntegerKind.U8 0) with (φ (Integer.Build_t IntegerKind.U8 0)).
+    apply array.repeat_nat_φ_eq.
+  Defined.
+  Global Opaque run_new_byte_str.
+
+  (* pub const fn from_str(s: &'static str) -> Arguments<'a> *)
+  Instance run_from_str (s : '& string) :
+    Run.Trait fmt.Impl_core_fmt_Arguments.from_str [] [] [φ s] Self.
   Proof.
     constructor.
     run_symbolic.
   Admitted.
-  Global Opaque run_new_v1.
+  Global Opaque run_from_str.
+
+  (* pub fn from_str_nonconst(s: &'static str) -> Arguments<'a> *)
+  Instance run_from_str_nonconst (s : '& string) :
+    Run.Trait fmt.Impl_core_fmt_Arguments.from_str_nonconst [] [] [φ s] Self.
+  Proof.
+    constructor.
+    run_symbolic.
+  Defined.
+  Global Opaque run_from_str_nonconst.
 End Impl_Arguments.
 Export (hints) Impl_Arguments.
